ott_coq/destination_calculus_sugar_typing.v
@@ -18,19 +18,19 @@ Require Import Arith.
 Require Import Dest.destination_calculus_proofs.
 Require Import Lia.
 
-Theorem Ty_term_termS_Alloc : forall (P : ctx) (T : type), DisposableOnly P -> P ⊢ alloc : T ⧔ (⌊ T ⌋ ¹ν).
+Theorem Ty_term_sterm_Alloc : forall (P : ctx) (T : type), DisposableOnly P -> P ⊢ alloc : T ⧔ (⌊ T ⌋ ¹ν).
 Proof.
   intros P T DisposP.
-  unfold termS_Alloc.
+  unfold sterm_Alloc.
   rewrite union_empty_r_eq with (G := P).
   apply Ty_term_Val.
   - assumption.
   - rewrite union_empty_r_eq with (G := ᴳ{}).
     assert (hvarsᴳ(ᴳ- ᴳ{+ 1 : ¹ν ⌊ T ⌋ ¹ν }) = ᴴ{ 1}) as hvarsD3Eq.
       { rewrite hvars_minus_eq. unfold hvars_ctx, hvars_dom, ctx_singleton, hminus. rewrite dom_singleton_eq. cbn. reflexivity. }
-    rewrite <- hvarsD3Eq. apply TyR_val_A; swap 1 10; swap 2 11.
-    + rewrite stimes_empty_eq, <- union_empty_l_eq. apply TyR_val_D.
-    + rewrite <- union_empty_l_eq. rewrite hminus_singleton. apply TyR_val_H.
+    rewrite <- hvarsD3Eq. apply Ty_val_Ampar; swap 1 10; swap 2 11.
+    + rewrite stimes_empty_eq, <- union_empty_l_eq. apply Ty_val_Dest.
+    + rewrite <- union_empty_l_eq. rewrite hminus_singleton. apply Ty_val_Hole.
     + apply DestOnly_singleton_dest.
     + apply LinOnly_singleton_iff. cbn. constructor.
     + apply FinAgeOnly_singleton_iff. cbn. constructor.
@@ -43,10 +43,10 @@ Proof.
   - + apply DestOnly_empty.
 Qed.
 
-Theorem Ty_term_termS_FromA' : forall (P : ctx) (t : term) (T : type), P ⊢ t : T ⧔ ① -> P ⊢ from⧔' t : T.
+Theorem Ty_term_sterm_FromA' : forall (P : ctx) (t : term) (T : type), P ⊢ t : T ⧔ ① -> P ⊢ from⧔' t : T.
 Proof.
   intros * Tyt.
-  unfold termS_FromA'.
+  unfold sterm_FromA'.
   replace P with (¹ν ᴳ· P ᴳ+ ᴳ{}). 2:{ crush. }
   apply Ty_term_PatP with (T1 := T) (T2 := ! ¹∞ ⁔ ①).
   - constructor.
@@ -60,7 +60,7 @@ Proof.
     + assumption.
     + rewrite stimes_empty_eq, union_commutative. apply Ty_term_PatU.
       * rewrite union_empty_l_eq with (G := ᴳ{ 0 : ¹ν ‗ ①}). apply Ty_term_Var. { apply DisposableOnly_empty. } { apply Disjoint_empty_l. } { repeat constructor. }
-      * rewrite union_empty_l_eq with (G := ᴳ{}). apply Ty_term_Val. { apply DisposableOnly_empty. } { rewrite <- stimes_empty_eq with (m := ¹∞). apply TyR_val_E. apply TyR_val_U. repeat constructor. } { apply DestOnly_empty. }
+      * rewrite union_empty_l_eq with (G := ᴳ{}). apply Ty_term_Val. { apply DisposableOnly_empty. } { rewrite <- stimes_empty_eq with (m := ¹∞). apply Ty_val_Exp. apply Ty_val_Unit. repeat constructor. } { apply DestOnly_empty. }
   - replace (ᴳ{} ᴳ+ ᴳ{ 1 : ¹ν ‗ T} ᴳ+ ᴳ{ 2 : ¹ν ‗ ! ¹∞ ⁔ ①}) with (¹ν ᴳ· ᴳ{ 2 : ¹ν ‗ ! ¹∞ ⁔ ①} ᴳ+ ᴳ{ 1 : ¹ν ‗ T}). 2:{ crush. }
     apply Ty_term_PatE with (T := ①).
     + repeat constructor.
@@ -72,24 +72,24 @@ Proof.
       * rewrite union_empty_l_eq with (G := ᴳ{ 1 : ¹ν ‗ T}). apply Ty_term_Var. { apply DisposableOnly_empty. }  { apply Disjoint_empty_l. } { repeat constructor. }
 Qed.
 
-Lemma Ty_term_termS_FillLeaf : forall (P1 P2 : ctx) (t t' : term) (T : type) (n : mode), IsValid n -> P1 ⊢ t : ⌊T⌋n -> P2 ⊢ t' : T -> P1 ᴳ+ (¹↑ · n) ᴳ·P2 ⊢ t ˢ⨞ t' : ①.
+Lemma Ty_term_sterm_FillLeaf : forall (P1 P2 : ctx) (t t' : term) (T : type) (n : mode), IsValid n -> P1 ⊢ t : ⌊T⌋n -> P2 ⊢ t' : T -> P1 ᴳ+ (¹↑ · n) ᴳ·P2 ⊢ t ˢ⨞ t' : ①.
 Proof.
   intros * Validn Tyt Tyt'.
-  unfold termS_FillLeaf.
+  unfold sterm_FillLeaf.
   replace (¹↑ · n) with (mode_times' ((¹↑ :: nil) ++ (n :: nil) ++ nil)). 2:{ cbn. destruct n; try destruct p; try destruct p2, a2; cbn; try destruct m, a; cbn; try rewrite Nat.add_0_r; trivial. }
-  apply Ty_term_FillC with (U := T); trivial.
+  apply Ty_term_FillComp with (U := T); trivial.
   apply Ty_term_ToA. assumption.
 Qed.
 
-Lemma Ty_term_termS_F : forall (P2 : ctx) (x: var) (m: mode) (u : term) (T U : type), UserDefined P2 -> IsValid m -> P2 # ᴳ{ x : m ‗ T} -> P2 ᴳ+ ᴳ{ x : m ‗ T} ⊢ u : U -> P2 ⊢ ˢλ x ⁔ m ⟼ u : T ⁔ m → U.
+Lemma Ty_term_sterm_Fun : forall (P2 : ctx) (x: var) (m: mode) (u : term) (T U : type), UserDefined P2 -> IsValid m -> P2 # ᴳ{ x : m ‗ T} -> P2 ᴳ+ ᴳ{ x : m ‗ T} ⊢ u : U -> P2 ⊢ ˢλ x ⁔ m ⟼ u : T ⁔ m → U.
 Proof.
   intros * UserDefinedP2 Validm DisjointP2x Tyu.
-  unfold termS_F.
-  apply Ty_term_termS_FromA'.
+  unfold sterm_Fun.
+  apply Ty_term_sterm_FromA'.
   rewrite union_empty_l_eq with (G := P2).
   apply Ty_term_Map with (T := ⌊T ⁔ m → U⌋ ¹ν).
   { apply UserDefined_Disjoint; trivial. lia. }
-  apply Ty_term_termS_Alloc. apply DisposableOnly_empty.
+  apply Ty_term_sterm_Alloc. apply DisposableOnly_empty.
   rewrite union_commutative.
   replace (¹↑) with (mode_times' ((¹↑ :: nil) ++ (¹ν :: nil) ++ nil)). 2:{ cbn. reflexivity. }
   apply Ty_term_FillF with (T := T) (U := U); trivial.
@@ -97,71 +97,71 @@ Proof.
   rewrite union_empty_l_eq with (G := ᴳ{ 0 : ¹ν ‗ ⌊ T ⁔ m → U ⌋ ¹ν}). apply Ty_term_Var. { apply DisposableOnly_empty. } { apply Disjoint_empty_l. } { repeat constructor. }
 Qed.
 
-Lemma Ty_term_termS_L : forall (P2 : ctx) (t : term) (T1 T2 : type), UserDefined P2 -> P2 ⊢ t : T1 -> P2 ⊢ ˢInl t : T1 ⨁ T2.
+Lemma Ty_term_sterm_Left : forall (P2 : ctx) (t : term) (T1 T2 : type), UserDefined P2 -> P2 ⊢ t : T1 -> P2 ⊢ ˢInl t : T1 ⨁ T2.
 Proof.
   intros * UserDefinedP2 Tyt.
-  unfold termS_L.
-  apply Ty_term_termS_FromA'.
+  unfold sterm_Left.
+  apply Ty_term_sterm_FromA'.
   rewrite union_empty_l_eq with (G := P2).
   apply Ty_term_Map with (T := ⌊T1 ⨁ T2⌋ ¹ν).
   { apply UserDefined_Disjoint; trivial. lia. }
-  apply Ty_term_termS_Alloc. apply DisposableOnly_empty.
+  apply Ty_term_sterm_Alloc. apply DisposableOnly_empty.
   rewrite union_commutative.
   replace (¹↑) with (¹↑ · ¹ν). 2:{ cbn. reflexivity. }
-  apply Ty_term_termS_FillLeaf with (T := T1); trivial.
+  apply Ty_term_sterm_FillLeaf with (T := T1); trivial.
   constructor.
   apply Ty_term_FillL with (T1 := T1) (T2 := T2); trivial.
   rewrite union_empty_l_eq with (G := ᴳ{ 0 : ¹ν ‗ ⌊ T1 ⨁ T2 ⌋ ¹ν}). apply Ty_term_Var. { apply DisposableOnly_empty. } { apply Disjoint_empty_l. } { repeat constructor. }
 Qed.
 
-Lemma Ty_term_termS_R : forall (P2 : ctx) (t : term) (T1 T2 : type), UserDefined P2 -> P2 ⊢ t : T2 -> P2 ⊢ ˢInr t : T1 ⨁ T2.
+Lemma Ty_term_sterm_Right : forall (P2 : ctx) (t : term) (T1 T2 : type), UserDefined P2 -> P2 ⊢ t : T2 -> P2 ⊢ ˢInr t : T1 ⨁ T2.
 Proof.
   intros * UserDefinedP2 Tyt.
-  unfold termS_R.
-  apply Ty_term_termS_FromA'.
+  unfold sterm_Right.
+  apply Ty_term_sterm_FromA'.
   rewrite union_empty_l_eq with (G := P2).
   apply Ty_term_Map with (T := ⌊T1 ⨁ T2⌋ ¹ν).
   { apply UserDefined_Disjoint; trivial. lia. }
-  apply Ty_term_termS_Alloc. apply DisposableOnly_empty.
+  apply Ty_term_sterm_Alloc. apply DisposableOnly_empty.
   rewrite union_commutative.
   replace (¹↑) with (¹↑ · ¹ν). 2:{ cbn. reflexivity. }
-  apply Ty_term_termS_FillLeaf with (T := T2); trivial.
+  apply Ty_term_sterm_FillLeaf with (T := T2); trivial.
   constructor.
   apply Ty_term_FillR with (T1 := T1) (T2 := T2); trivial.
   rewrite union_empty_l_eq with (G := ᴳ{ 0 : ¹ν ‗ ⌊ T1 ⨁ T2 ⌋ ¹ν}). apply Ty_term_Var. { apply DisposableOnly_empty. } { apply Disjoint_empty_l. } { repeat constructor. }
 Qed.
 
-Lemma Ty_term_termS_E : forall (P2 : ctx) (m : mode) (t : term) (T : type), UserDefined P2 -> IsValid m -> P2 ⊢ t : T -> m ᴳ· P2 ⊢ ˢᴇ m ⁔ t : ! m ⁔ T.
+Lemma Ty_term_sterm_Exp : forall (P2 : ctx) (m : mode) (t : term) (T : type), UserDefined P2 -> IsValid m -> P2 ⊢ t : T -> m ᴳ· P2 ⊢ ˢᴇ m ⁔ t : ! m ⁔ T.
 Proof.
   intros * UserDefinedP2 Validm Tyt.
-  unfold termS_E.
-  apply Ty_term_termS_FromA'.
+  unfold sterm_Exp.
+  apply Ty_term_sterm_FromA'.
   rewrite union_empty_l_eq with (G := m ᴳ· P2).
   apply Ty_term_Map with (T := ⌊! m ⁔ T⌋ ¹ν).
   { apply UserDefined_Disjoint; trivial.
     unfold UserDefined in *. intros x. specialize (UserDefinedP2 x). unfold stimes. rewrite In_map_iff. assumption.
     lia. }
-  apply Ty_term_termS_Alloc. apply DisposableOnly_empty.
+  apply Ty_term_sterm_Alloc. apply DisposableOnly_empty.
   rewrite union_commutative.
   rewrite stimes_is_action.
-  apply Ty_term_termS_FillLeaf with (P2 := P2) (T := T); trivial.
+  apply Ty_term_sterm_FillLeaf with (P2 := P2) (T := T); trivial.
   replace (⌊ T ⌋ m) with (⌊ T ⌋ mode_times' ((m :: nil) ++ (¹ν :: nil) ++ nil)). 2: { f_equal. cbn. apply mode_times_linnu_r_eq. }
   apply Ty_term_FillE.
   constructor.
   rewrite union_empty_l_eq with (G := ᴳ{ 0 : ¹ν ‗ ⌊ ! m ⁔ T ⌋ ¹ν}). apply Ty_term_Var. { apply DisposableOnly_empty. } { apply Disjoint_empty_l. } { repeat constructor. }
 Qed.
 
-Lemma Ty_term_termS_P : forall (P21 P22 : ctx) (t1 t2 : term) (T1 T2 : type), UserDefined P21 -> UserDefined P22 -> P21 ⊢ t1 : T1 -> P22 ⊢ t2 : T2 -> (P21 ᴳ+ P22) ⊢ ˢ(t1, t2) : T1 ⨂ T2.
+Lemma Ty_term_sterm_Prod : forall (P21 P22 : ctx) (t1 t2 : term) (T1 T2 : type), UserDefined P21 -> UserDefined P22 -> P21 ⊢ t1 : T1 -> P22 ⊢ t2 : T2 -> (P21 ᴳ+ P22) ⊢ ˢ(t1, t2) : T1 ⨂ T2.
 Proof.
   intros * UserDefinedP21 UserDefinedP22 Tyt1 Tyt2.
   assert (UserDefined (P21 ᴳ+ P22)).
   { apply UserDefined_union_iff. split; assumption. }
-  unfold termS_P.
-  apply Ty_term_termS_FromA'.
+  unfold sterm_Prod.
+  apply Ty_term_sterm_FromA'.
   rewrite union_empty_l_eq with (G := P21 ᴳ+ P22).
   apply Ty_term_Map with (T := ⌊T1 ⨂ T2⌋ ¹ν).
   { apply UserDefined_Disjoint; trivial. lia. }
-  apply Ty_term_termS_Alloc. apply DisposableOnly_empty.
+  apply Ty_term_sterm_Alloc. apply DisposableOnly_empty.
   rewrite union_commutative.
   replace (ᴳ{ 0 : ¹ν ‗ ⌊ T1 ⨂ T2 ⌋ ¹ν}) with (¹ν ᴳ· ᴳ{ 0 : ¹ν ‗ ⌊ T1 ⨂ T2 ⌋ ¹ν}). 2:{ rewrite stimes_linnu_eq. reflexivity. }
   apply Ty_term_PatP with (T1 := ⌊ T1 ⌋ ¹ν) (T2 := ⌊ T2 ⌋ ¹ν).
@@ -177,23 +177,23 @@ Proof.
   replace (¹↑ ᴳ· (P21 ᴳ+ P22) ᴳ+ ᴳ{ 1 : ¹ν ‗ ⌊ T1 ⌋ ¹ν} ᴳ+ ᴳ{ 2 : ¹ν ‗ ⌊ T2 ⌋ ¹ν}) with ((ᴳ{ 1 : ¹ν ‗ ⌊ T1 ⌋ ¹ν} ᴳ+ ¹↑ ᴳ· P21) ᴳ+ (ᴳ{ 2 : ¹ν ‗ ⌊ T2 ⌋ ¹ν} ᴳ+ ¹↑ ᴳ· P22)). 2:{ rewrite stimes_distrib_on_union. rewrite union_commutative with (G1 := ᴳ{ 1 : ¹ν ‗ ⌊ T1 ⌋ ¹ν}). rewrite union_associative. rewrite <- union_associative with (G1 := ¹↑ ᴳ· P21). rewrite <- union_associative. rewrite union_commutative with (G1 := ᴳ{ 1 : ¹ν ‗ ⌊ T1 ⌋ ¹ν} ᴳ+ ᴳ{ 2 : ¹ν ‗ ⌊ T2 ⌋ ¹ν}). crush. }
   apply Ty_term_PatU;
   replace (¹↑) with (¹↑ · ¹ν); try (cbn; reflexivity).
-  apply Ty_term_termS_FillLeaf with (P2 := P21) (T := T1); trivial.
+  apply Ty_term_sterm_FillLeaf with (P2 := P21) (T := T1); trivial.
   constructor.
   rewrite union_empty_l_eq with (G := ᴳ{ 1 : ¹ν ‗ ⌊ T1 ⌋ ¹ν}). apply Ty_term_Var. { apply DisposableOnly_empty. } { apply Disjoint_empty_l. } { repeat constructor. }
-  apply Ty_term_termS_FillLeaf with (P2 := P22) (T := T2); trivial.
+  apply Ty_term_sterm_FillLeaf with (P2 := P22) (T := T2); trivial.
   constructor.
   rewrite union_empty_l_eq with (G := ᴳ{ 2 : ¹ν ‗ ⌊ T2 ⌋ ¹ν}). apply Ty_term_Var. { apply DisposableOnly_empty. } { apply Disjoint_empty_l. } { repeat constructor. }
 Qed.
 
-Theorem Ty_termS_coherency : forall (P : ctx) (t : term) (T : type), P ˢ⊢ t : T -> P ⊢ t : T.
+Theorem Ty_sterm_coherency : forall (P : ctx) (t : term) (T : type), P ˢ⊢ t : T -> P ⊢ t : T.
 Proof.
   intros * Tyst. inversion Tyst; subst. inversion Tyst; subst.
-  - apply Ty_term_termS_Alloc; trivial.
-  - apply Ty_term_termS_FromA'; trivial.
-  - replace (mode_times' ((¹↑ :: nil) ++ (n :: nil) ++ nil)) with (¹↑ · n). 2:{ cbn. destruct n; try destruct p; try destruct p2, a2; cbn; try destruct m, a; cbn; try rewrite Nat.add_0_r; trivial. } apply Ty_term_termS_FillLeaf with (T := T0); trivial.
-  - apply Ty_term_termS_F; trivial.
-  - apply Ty_term_termS_L; trivial.
-  - apply Ty_term_termS_R; trivial.
-  - apply Ty_term_termS_E; trivial.
-  - apply Ty_term_termS_P; trivial.
+  - apply Ty_term_sterm_Alloc; trivial.
+  - apply Ty_term_sterm_FromA'; trivial.
+  - replace (mode_times' ((¹↑ :: nil) ++ (n :: nil) ++ nil)) with (¹↑ · n). 2:{ cbn. destruct n; try destruct p; try destruct p2, a2; cbn; try destruct m, a; cbn; try rewrite Nat.add_0_r; trivial. } apply Ty_term_sterm_FillLeaf with (T := T0); trivial.
+  - apply Ty_term_sterm_Fun; trivial.
+  - apply Ty_term_sterm_Left; trivial.
+  - apply Ty_term_sterm_Right; trivial.
+  - apply Ty_term_sterm_Exp; trivial.
+  - apply Ty_term_sterm_Prod; trivial.
 Qed.
